Reorderer/Impl.v
@@ -17,6 +17,11 @@ Section Reorderer.
 
       enqPtr: string;
       deqPtr: string;
+
+      validArray: string;
+
+      logNumReqId: nat;
+      lenIsPow2: Nat.pow 2 logNumReqId = numReqId;
     }.
 
   Section withParams.
@@ -24,8 +29,17 @@ Section Reorderer.
     Local Open Scope kami_expr.
     Local Open Scope kami_action.
 
-    Definition reqIdLen := Nat.pow 2 reqIdSz.
+    Lemma logNumReqId_reqIdSz: logNumReqId = reqIdSz.
+    Proof.
+      unfold reqIdSz.
+      rewrite <- lenIsPow2.
+      rewrite Nat.log2_up_pow2; auto; try Omega.omega.
+    Qed.
+
+    Definition castToReqIdSz (t: nat -> Type) (val: t logNumReqId): t reqIdSz :=
+      eq_rect logNumReqId t val reqIdSz logNumReqId_reqIdSz.
     
+    Definition ReordererPtr := Bit (logNumReqId + 1).
     Section withTy.
 
       (* Conceptual rule *)
@@ -35,16 +49,19 @@ Section Reorderer.
       : ActionT ty Void
         := Read deqPFull: ReordererPtr <- deqPtr;
            Read enqPFull: ReordererPtr <- enqPtr;
-           LET deqP: ReordererReqId <- UniBit (TruncLsb _ 1) #deqPFull;
-           Call inst: Maybe MInst <- rfRead(#deqP: ReordererReqId);
+           Read valids: Array numReqId Bool <- validArray;
+           LET deqP: ReordererReqId
+                       <- UniBit (TruncLsb _ 1)
+                       (castToReqIdSz (fun n => Expr ty (SyntaxKind (Bit (n + 1)))) #deqPFull);
+           Call inst: MInst <- rfRead(#deqP: ReordererReqId);
            Call vaddr: VAddr <- arfRead(#deqP: ReordererReqId);
            LET resp
            :  ReordererRes
                 <- STRUCT {
                   "vaddr" ::= #vaddr;
-                  "inst"  ::= #inst @% "data"
+                  "inst"  ::= #inst
                 };
-           If (#deqPFull != #enqPFull) && #inst @% "valid"
+           If (#deqPFull != #enqPFull) && (#valids@[#deqP])
            then
              LETA _ <- prefetcherCallback (resp : ty ReordererRes);
              Write deqPtr <- #deqPFull + $1;
@@ -56,8 +73,10 @@ Section Reorderer.
       Definition reordererCallback ty (resp: ty ReordererArbiterRes): ActionT ty Void :=
         LET idx: ReordererReqId <- #resp @% "tag";
         LET res: MInst <- #resp @% "resp";
+        Read valids: Array numReqId Bool <- validArray;
+        Write validArray: Array numReqId Bool <- #valids@[#idx <- $$true];
         Call rfWrite(STRUCT { "addr" ::= #idx;
-                              "data" ::= Valid #res } : WriteRq reqIdSz (Maybe MInst));
+                              "data" ::= #res } : WriteRq reqIdSz MInst);
         Retv.
 
       Definition sendReq
@@ -69,8 +88,11 @@ Section Reorderer.
         :  ActionT ty ReordererImmRes
         := Read enqPFull: ReordererPtr <- enqPtr;
            Read deqPFull: ReordererPtr <- deqPtr;
-           LET enqP: ReordererReqId <- UniBit (TruncLsb _ 1) #enqPFull;
-           LET deqP: ReordererReqId <- UniBit (TruncLsb _ 1) #deqPFull;
+           Read valids: Array numReqId Bool <- validArray;
+           LET enqP: ReordererReqId <- UniBit (TruncLsb _ 1)
+                                    (castToReqIdSz (fun n => Expr ty (SyntaxKind (Bit (n + 1)))) #enqPFull);
+           LET deqP: ReordererReqId <- UniBit (TruncLsb _ 1)
+                                    (castToReqIdSz (fun n => Expr ty (SyntaxKind (Bit (n + 1)))) #deqPFull);
            LET arbiterReq
            :  ReordererArbiterReq
                 <- STRUCT {
@@ -83,8 +105,7 @@ Section Reorderer.
              If #res @% "ready"
              then
                Write enqPtr <- #enqPFull + $1;
-               Call rfWrite(STRUCT { "addr" ::= #enqP;
-                                     "data" ::= Invalid } : WriteRq reqIdSz (Maybe MInst));
+               Write validArray: Array numReqId Bool <- #valids@[#enqP <- $$false];
                Call arfWrite
                  (STRUCT {
                     "addr" ::= #enqP;
@@ -105,12 +126,13 @@ Section Reorderer.
     Open Scope kami_expr_scope.
     
     Definition regs: list RegInitT := makeModule_regs ( Register enqPtr: ReordererPtr <- $ 0 ++
-                                                        Register deqPtr: ReordererPtr <- $ 0 ).
+                                                        Register deqPtr: ReordererPtr <- $ 0 ++
+                                                        RegisterU validArray: Array numReqId Bool                                                                  ).
 
     Definition regFiles: list RegFileBase :=
       [ 
         @Build_RegFileBase false 1 rfName
-                           (Async [rfRead]) rfWrite reqIdSz (Maybe MInst) (@RFNonFile _ _ None);
+                           (Async [rfRead]) rfWrite reqIdSz MInst (@RFNonFile _ _ None);
           
         @Build_RegFileBase false 1 arfName
                            (Async [arfRead]) arfWrite reqIdSz VAddr (@RFNonFile _ _ None)
